theories/soundness/getc.v
@@ -23,39 +23,38 @@ Section proofs.
   (* Iris semantic context *)
   Context `{!sem_heapGS Θ}.
 
-  Lemma get_priv_soundness C Δ rigid Γ lhs t σ name fty:
+  (*
+  Lemma get_priv_soundness C cdef Δ rigid Γ lhs name fty:
     wf_cdefs pdefs →
     wf_lty Γ →
-    type_of_this Γ = (t, σ) →
-    has_field name t Private fty C →
-    ∀ Σ st st' n,
+    pdefs !! C = Some cdef →
+    has_field name C Private fty C →
+    ∀ Σthis Σ st st' n,
     length Σ = rigid →
     cmd_eval C st (GetC lhs ThisE name) st' n →
+    □ interp_as_mixed Σthis -∗
+    interp_inclusion Σthis (interp_tag_alt C Σ) -∗
     □ interp_env_as_mixed Σ -∗
-    □ Σinterp Σ Δ -∗
-    heap_models st.2 ∗ interp_local_tys Σ Γ st.1 -∗
-    |=▷^n heap_models st'.2 ∗ interp_local_tys Σ (<[lhs:=subst_ty σ fty]> Γ) st'.1.
+    □ Σinterp Σthis Σ Δ -∗
+    heap_models st.2 ∗ interp_local_tys Σthis Σ Γ st.1 -∗
+    |=▷^n heap_models st'.2 ∗ interp_local_tys Σthis Σ (<[lhs:=fty]> Γ) st'.1.
   Proof.
-    move => wfpdefs wflty hthis hf Σ st st' n hrigid hc.
-    iIntros "hΣ hΣΔ".
+    move => wfpdefs wflty hcdef hf Σthis Σ st st' n hrigid hc.
+    iIntros "#hΣthis hΣthis_incl #hΣ #hΣΔ".
     elim/cmd_eval_getI: hc.
     move => {n}.
     move => Ω h l t0 vs v heval hheap hvs hvis.
-    iIntros "[Hh #Hle]".
+    iIntros "[Hh Hle]".
     iModIntro. (* keep the later *)
-    destruct Γ as [[this thisσ] Γ].
     destruct Ω as [vthis Ω].
-    destruct wflty as [wfthis wflty].
-    rewrite /this_type /= in wfthis, hthis.
-    injection hthis; intros; subst; clear hthis.
     case: heval => ->.
     simpl in *.
-    iDestruct "Hle" as "[Hthis Hle]".
-    rewrite /this_type /=.
-    rewrite /interp_this_type interp_this_unseal /interp_this_def /=.
-    iDestruct "Hthis" as (??? σ0 ???) "(%H & #hmixed & #? & %hinst & #hdyn & H◯)".
-    destruct H as ([= <-] & hdef1 & ? & hinherits & hidom & hfields).
-    iAssert (⌜t0 = t1⌝ ∗ heap_models h ∗ ▷ interp_type (subst_ty σ fty) Σ v)%I with "[Hh]" as "[%Ht [Hh Hv]]".
+    iDestruct "Hle" as "[Hthis #Hle]" => /=.
+    iDestruct ("hΣthis_incl" with "Hthis") as "#h".
+    iDestruct "h" as (???? σ0 ???) "(%H & #hmixed & #? & #hinst & #hdyn & H◯)".
+    destruct H as ([= <-] & ? & htdef & hlen & hinherits & hidom & hfields).
+    simplify_eq.
+    iAssert (⌜t0 = t⌝ ∗ heap_models h ∗ ▷ interp_type (subst_gen C cdef fty) Σthis Σ v)%I with "[Hh]" as "[%Ht [Hh Hv]]".
     { iDestruct "Hh" as (sh) "(H● & %hdom & #Hh)".
       iDestruct (sem_heap_own_valid_2 with "H● H◯") as "#HΦ".
       iDestruct ("Hh" with "[//]") as (iFs) "[H H▷]".
@@ -65,7 +64,7 @@ Section proofs.
       fold_leibniz; subst.
       iSplitR; first done.
       iSplitL. { iExists _. iFrame. by iSplit. }
-      assert (hfC: has_field name t1 Private (subst_ty σ0 fty) C) by (destruct wfpdefs; by eapply has_field_inherits_using).
+      assert (hfC: has_field name t Private (subst_ty σ0 fty) C) by (destruct wfpdefs; by eapply has_field_inherits_using).
       iSpecialize ("hdyn" $! name Private (subst_ty σ0 fty) C hfC).
       iDestruct "H▷" as "[hdf h]".
       rewrite later_equivI. iNext.
@@ -73,15 +72,21 @@ Section proofs.
       iSpecialize ("h" $! name _ with "[hdyn]"); first done.
       iDestruct "h" as (w) "[%hw hiw]".
       simplify_eq.
+
+      iAssert (interp_type (subst_ty σ0 fty) (interp_exact_class interp_type t Σt) Σt v) as "#Ht".
+      { by rewrite /subst_gen -hlen -interp_type_subst_this. }
+      iClear "hiw".
+
       rewrite interp_type_subst; last first.
       { destruct wfpdefs.
         apply has_field_bounded in hf => //.
         destruct hf as (? & ? & ?).
         apply inherits_using_wf in hinherits => //.
-        destruct hinherits as (? & ?& ? & hh).
-        apply wf_tyI in wfthis as (? & ? & hlen & ?); simplify_eq.
-        by rewrite hlen.
+        destruct hinherits as (? & ?& ? & hh & _).
+        apply wf_tyI in hh as (? & ? & hlenC & ?); simplify_eq.
+        by rewrite hlenC.
       }
+
       rewrite -hinst.
       rewrite -interp_type_subst //.
       destruct wfpdefs.
@@ -101,50 +106,146 @@ Section proofs.
     iExists l, t1, tdef, σ0, Σt, fields, ifields.
     by repeat iSplit.
   Qed.
+   *)
 
   Lemma get_pub_soundness C Δ kd rigid Γ lhs recv exact_ t σ name fty orig:
     wf_cdefs pdefs →
     wf_lty Γ →
     Forall wf_constraint Δ →
     expr_has_ty Δ Γ rigid kd recv (ClassT exact_ t σ) →
-    has_field name t Public fty orig →
-    ∀ Σ st st' n,
+    field_lookup exact_ t σ name Public fty orig →
+    ∀ Σthis Σ st st' n,
     length Σ = rigid →
     cmd_eval C st (GetC lhs recv name) st' n →
+    □ interp_as_mixed Σthis -∗
     □ interp_env_as_mixed Σ -∗
-    □ Σinterp Σ Δ -∗
-    heap_models st.2 ∗ interp_local_tys Σ Γ st.1 -∗
-    |=▷^n heap_models st'.2 ∗ interp_local_tys Σ (<[lhs:=subst_ty σ fty]> Γ) st'.1.
+    □ Σinterp Σthis Σ Δ -∗
+    heap_models st.2 ∗ interp_local_tys Σthis Σ Γ st.1 -∗
+    |=▷^n heap_models st'.2 ∗ interp_local_tys Σthis Σ (<[lhs:=subst_fty exact_ t σ fty]> Γ) st'.1.
   Proof.
-    move => wfpdefs ?? hrecv hf Σ st st' n hrigid hc.
-    iIntros "hΣ hΣΔ".
+    move => wfpdefs ?? hrecv hf Σthis Σ st st' n hrigid hc.
+    iIntros "hΣthis hΣ hΣΔ".
     elim/cmd_eval_getI: hc.
     move => {n}.
     move => Ω h l t0 vs v heval hheap hvs hvis.
     iIntros "[Hh #Hle]".
     iModIntro. (* keep the later *)
-    iDestruct (expr_soundness with "hΣ hΣΔ Hle") as "He" => //; try (by apply wfpdefs).
-    iDestruct (exact_subtype_is_inclusion with "He") as "He".
-    rewrite interp_class_unfold //; first last.
-    { apply expr_has_ty_wf in hrecv => //.
-      by eapply wf_ty_exact.
-    }
-    { by apply wfpdefs. }
-    iDestruct "He" as (?? def def0 σ0 ???) "(%H & #hmixed & #? & #hf0 & #hdyn & #H◯)".
-    destruct H as ([= <-] & hdef & hdef0 & ? & hinherits & hfields & hidom).
     assert (hwf0: wf_ty (ClassT exact_ t σ)) by (by apply expr_has_ty_wf in hrecv).
-    assert (hl0: length (generics def) = length σ0).
+    assert (hwf0_ := hwf0).
+    apply wf_tyI in hwf0_ as (tdef & htdef & hlen & hfσ); simplify_eq.
+    iDestruct (expr_soundness with "hΣthis hΣ hΣΔ Hle") as "He" => //; try (by apply wfpdefs).
+    destruct hf as [hf hex].
+    case: hex => [h_is_exact | hnothis_t ].
+    (* receiver class is exact *)
+    - rewrite /is_true in h_is_exact; simplify_eq.
+      rewrite interp_exact_class_unfold; first last.
+      { by assumption. }
+      { by apply wfpdefs. }
+      iDestruct "He" as (tdef' Σt H)"(#hmixed & #hinst & #htag)".
+      destruct H as [htdef' hΣtlen]; simplify_eq.
+      iDestruct "htag" as (l0 tdef' fields ifields H) "(#hconstr & hf0 & #H◯)".
+      destruct H as ([= <-] & htdef' & hfields & hidom); simplify_eq.
+      simpl.
+      iAssert (⌜t0 = t⌝ ∗ heap_models h ∗
+        ▷ interp_type (subst_gen t tdef fty) interp_nothing Σt v)%I with "[Hh]" as "[%Ht [Hh Hv]]".
+      { iDestruct "Hh" as (sh) "(H● & %hdom & #Hh)".
+        iDestruct (sem_heap_own_valid_2 with "H● H◯") as "#HΦ".
+        iDestruct ("Hh" with "[//]") as (iFs) "[H H▷]".
+        iRewrite "H" in "HΦ".
+        rewrite option_equivI prod_equivI /=.
+        iDestruct "HΦ" as "[%Ht HΦ]".
+        fold_leibniz; subst.
+        iSplitR; first done.
+        iSplitL. { iExists _. iFrame. by iSplit. }
+        iSpecialize ("hf0" $! name Public fty orig hf).
+        iNext.
+        iDestruct "H▷" as "[%hdf h]".
+        iRewrite -"HΦ" in "hf0".
+        iSpecialize ("h" $! name _ with "[hf0]"); first done.
+        iDestruct "h" as (w) "[%hw hiw]".
+        by simplify_eq.
+      }
+      subst; simpl.
+      iNext.
+      iFrame.
+      destruct wfpdefs.
+      iApply interp_local_tys_update => //.
+      rewrite /subst_gen /subst_fty -hΣtlen.
+      rewrite interp_type_subst_this => //.
+      rewrite interp_type_subst; last first.
+      { apply has_field_bounded in hf => //.
+        destruct hf as (?&?&hf); simplify_eq.
+        apply bounded_subst_this.
+        + by rewrite hlen.
+        + constructor.
+          by apply bounded_gen_targs.
+      }
+      replace (length σ) with (length (interp_list Σthis Σ σ)) by by rewrite /interp_list map_length.
+      rewrite interp_type_subst_this; first last.
+      { by rewrite /interp_list map_length. }
+      { by assumption. }
+
+      t tdef Σthis (interp_list Σthis Σ σ) fty v htdef).
+      rewrite hlen interp_type_subst_this.
+      rewrite (interp_list_no_this _ _ (interp_exact_class interp_type t1 Σt) interp_nothing); last done.
+    iAssert (interp_type fty (interp_exact_class interp_type t1 Σt)
+                (interp_list Σthis Σ σ) v) with "[Hv]" as "Hv".
+    { iApply interp_with_mono => //.
+      - apply has_field_mono in hf => //.
+        destruct hf as (?&?&hh); simplify_eq.
+        by destruct hh.
+      - by apply has_field_wf in hf.
+    }
+    - destruct exact_; last done.
+      clear h_is_exact.
+      rewrite interp_type_subst; last first.
+      { apply bounded_subst_this.
+        - apply has_field_bounded in hf => //.
+          destruct hf as (?&?&hf); simplify_eq.
+          by rewrite -hl1 -hl0.
+        - constructor.
+          by apply bounded_gen_targs.
+      }
+      replace (length σ) with (length (interp_list Σthis Σ σ)) by by rewrite /interp_list map_length.
+      rewrite (interp_type_subst_this t tdef); first last.
+      { by rewrite /interp_list map_length hlen. }
+      { done. }
+      (* ARGL *)
+
+
+
+
+
+
+
+
+
+
+
+
+
+    rewrite interp_tag_unfold interp_tag_equiv; first last.
+    { by rewrite /interp_list fmap_length. }
+    { done. }
+    { by apply wfpdefs. }
+    iDestruct "He" as (?? def def1 σ0 ???) "(%H & #hmixed & #? & #hf0 & #hdyn & #H◯)".
+    destruct H as ([= <-] & hdef & hdef1 & hlenΣt & hinherits & hfields & hidom).
+    assert (hl0: length (generics def) = length σ0 ∧ 
+                 Forall (λ ty : lang_ty, no_this ty) σ0).
     { apply inherits_using_wf in hinherits; try (by apply wfpdefs).
-      destruct hinherits as (?&?&?&hh).
+      destruct hinherits as (?&?&?&hh&hnothis).
       apply wf_tyI in hh as (? & ? & ? & ?); by simplify_eq.
     }
+    destruct hl0 as [hl0 hnothis].
     assert (hl1: length σ0 = length σ).
     { rewrite -hl0.
       apply wf_tyI in hwf0 as (? & ? & ? & ?); by simplify_eq.
     }
     assert (hff: has_field name t1 Public (subst_ty σ0 fty) orig).
     { by apply has_field_inherits_using with (A := t1) (σB := σ0) in hf => //; try (by apply wfpdefs). }
-    iAssert (⌜t0 = t1⌝ ∗ heap_models h ∗ ▷ interp_type (subst_ty σ0 fty) Σt v)%I with "[Hh]" as "[%Ht [Hh Hv]]".
+    simpl.
+    iAssert (⌜t0 = t1⌝ ∗ heap_models h ∗
+      ▷ interp_type (subst_gen t1 def1 (subst_ty σ0 fty)) interp_nothing Σt v)%I with "[Hh]" as "[%Ht [Hh Hv]]".
     { iDestruct "Hh" as (sh) "(H● & %hdom & #Hh)".
       iDestruct (sem_heap_own_valid_2 with "H● H◯") as "#HΦ".
       iDestruct ("Hh" with "[//]") as (iFs) "[H H▷]".
@@ -167,20 +268,66 @@ Section proofs.
     iFrame.
     destruct wfpdefs.
     iApply interp_local_tys_update => //.
-    rewrite !interp_type_subst; first last.
+    rewrite /subst_gen /subst_fty -hlenΣt.
+    rewrite interp_type_subst_this => //.
+    rewrite interp_type_subst; last first.
     { apply has_field_bounded in hf => //.
       destruct hf as (?&?&hf); simplify_eq.
       by rewrite -hl0.
     }
-    { apply has_field_bounded in hf => //.
-      destruct hf as (?&?&hf); simplify_eq.
-      by rewrite -hl1 -hl0.
+    rewrite (interp_list_no_this _ _ (interp_exact_class interp_type t1 Σt) interp_nothing); last done.
+    iAssert (interp_type fty (interp_exact_class interp_type t1 Σt)
+                (interp_list Σthis Σ σ) v) with "[Hv]" as "Hv".
+    { iApply interp_with_mono => //.
+      - apply has_field_mono in hf => //.
+        destruct hf as (?&?&hh); simplify_eq.
+        by destruct hh.
+      - by apply has_field_wf in hf.
     }
-    iApply interp_with_mono => //.
-    { apply has_field_mono in hf => //.
-      destruct hf as (?&?&hh); simplify_eq.
-      by destruct hh.
-    }
-    by apply has_field_wf in hf.
+    - destruct exact_; last done.
+      clear h_is_exact.
+      rewrite interp_type_subst; last first.
+      { apply bounded_subst_this.
+        - apply has_field_bounded in hf => //.
+          destruct hf as (?&?&hf); simplify_eq.
+          by rewrite -hl1 -hl0.
+        - constructor.
+          by apply bounded_gen_targs.
+      }
+      replace (length σ) with (length (interp_list Σthis Σ σ)) by by rewrite /interp_list map_length.
+      rewrite (interp_type_subst_this t tdef); first last.
+      { by rewrite /interp_list map_length hlen. }
+      { done. }
+      (* ARGL *)
+
+
+    (* ONLY WORKS if t has no this *)
+    rewrite (interp_type_no_this _ _ _ Σthis interp_nothing); first last.
+    { apply wf_tyI in hwf0.
+      apply subst_ty_has_no_this.
+      - apply subst_this_has_no_this => /=.
+        simp
+        rewrite subst_this_no_this_id.
+
+
+    - assert (hfty_nothis: no_this fty) by admit.
+      rewrite subst_this_no_this_id; last admit.
+      rewrite subst_this_no_this_id; last done.
+      rewrite !interp_type_subst; first last.
+      { apply has_field_bounded in hf => //.
+        destruct hf as (?&?&hf); simplify_eq.
+        by rewrite -hl0.
+      }
+      { apply has_field_bounded in hf => //.
+        destruct hf as (?&?&hf); simplify_eq.
+        by rewrite -hl1 -hl0.
+      }
+      rewrite (interp_type_no_this _ fty v interp_nothing Σthis hfty_nothis).
+      iApply interp_with_mono => //.
+      { apply has_field_mono in hf => //.
+        destruct hf as (?&?&hh); simplify_eq.
+        by destruct hh.
+      }
+      by apply has_field_wf in hf.
   Qed.
 End proofs.
