theories/this_examples.v
@@ -1,0 +1,405 @@
+(*
+ * Copyright (c) Meta Platforms, Inc. and affiliates.
+ *
+ * This source code is licensed under the MIT license found in the
+ * LICENSE file in the root directory of this source tree.
+ *)
+From stdpp Require Import base strings gmap stringmap fin_maps.
+
+From iris.proofmode Require Import tactics.
+From iris.base_logic.lib Require Import iprop own wsat.
+From iris.algebra.lib Require Import gmap_view.
+
+From shack Require Import lang progdef subtype ok typing.
+From shack Require Import eval heap.
+
+Definition arraykey := UnionT IntT BoolT.
+
+(* Definition of class C:
+ * class C {
+ *   function f(this $_): void {}
+ *)
+Definition f := {|
+  methodargs := {[ "$in" := ThisT ]};
+  methodrettype := NullT;
+  methodbody := SkipC;
+  methodret := NullE;
+  methodvisibility := Public;
+|}.
+
+Definition C := {|
+  superclass := None;
+  generics := [];
+  constraints := [];
+  classfields := ∅;
+  classmethods := {["f" := f]};
+|}.
+
+(* TODO simpl g *)
+(* Definition of class D:
+ * class D extends C {
+ *   function f(this $in): void {
+        $in->g(in);
+   }
+ *   function g(this $_): void {}
+ *)
+Definition f2 := {|
+  methodargs := {[ "$in" := ThisT ]};
+  methodrettype := NullT;
+  methodbody := CallC "$_" (VarE "$in") "g" {[ "$in" := VarE "$in" ]};
+  methodret := NullE;
+  methodvisibility := Public;
+|}.
+
+Definition g := f.
+
+Definition D := {|
+  superclass := Some ("C", []);
+  generics := [];
+  constraints := [];
+  classfields := ∅;
+  classmethods := {["f" := f2; "g" := g]};
+|}.
+
+(* Main program:
+    function problem(C $c0, C $c1) : void {
+      $r = $c0->f($c1);
+   }
+
+    function main(): void {
+      problem(new D(), new C());
+    }
+*)
+Definition MainBody :=
+   SeqC (NewC "$d" "D" (Some []) ∅)
+  (SeqC (NewC "$c" "C" (Some []) ∅)
+        (CallC "$tmp" ThisE "problem" {[ "$c0" := VarE "$d"; "$c1" := VarE "$c"]}))
+  .
+
+Definition problem := {|
+  methodargs := {[ "$c0" := ClassT false "C" []; "$c1" := ClassT false "C" [] ]};
+  methodrettype := NullT;
+  methodbody := CallC "$_" (VarE "$c0") "f" {[ "$in" := VarE "$c1" ]};
+  methodret := NullE;
+  methodvisibility := Public;
+|}.
+
+Definition main := {|
+  methodargs := ∅;
+  methodrettype := NullT;
+  methodbody := MainBody;
+  methodret := NullE;
+  methodvisibility := Public;
+|}.
+
+Definition Main := {|
+  superclass := None;
+  generics := [];
+  constraints := [];
+  classfields := ∅;
+  classmethods := {["main" := main; "problem" := problem ]}
+ |}.
+
+Local Instance PDC : ProgDefContext := { pdefs := {[ "C" := C; "D" := D; "Main" := Main ]} }.
+
+Lemma pacc : ∀ c : tag, Acc (λ x y : tag, extends y x) c.
+Proof.
+  assert (helperC: Acc (λ x y : tag, extends y x) "C").
+  { constructor => t hext.
+    inv hext.
+    rewrite lookup_insert in H; case: H => H; by simplify_eq.
+  }
+  assert (helper: Acc (λ x y : tag, extends y x) "D").
+  { constructor => t hext.
+    inv hext.
+    rewrite lookup_insert_ne in H; last done.
+    rewrite lookup_insert in H; case: H => H; subst.
+    rewrite /D /= in H0; by simplify_eq.
+  }
+  move => c.
+  destruct (String.eqb c "C") eqn:heq0.
+  { by apply String.eqb_eq in heq0 as ->. }
+  apply String.eqb_neq in heq0.
+  destruct (String.eqb c "D") eqn:heq1.
+  { by apply String.eqb_eq in heq1 as ->. }
+  apply String.eqb_neq in heq1.
+  destruct (String.eqb c "Main") eqn: heq2.
+  { apply String.eqb_eq in heq2 as ->.
+    constructor => t hext.
+    inv hext.
+    rewrite lookup_insert_ne in H; last done.
+    rewrite lookup_insert_ne in H; last done.
+    rewrite lookup_insert in H; case: H => H; subst.
+    by rewrite /Main /= in H0.
+  }
+  apply String.eqb_neq in heq2.
+  constructor => t hext; exfalso.
+  inv hext.
+  by repeat (rewrite lookup_insert_ne // in H).
+Qed.
+
+Local Instance PDA : ProgDefAcc  := { pacc := pacc }.
+
+(* Invalid constraint, so we can prove anything trivially *)
+Local Instance SDTCC : SDTClassConstraints := {
+  Δsdt := λ _, [(IntT, BoolT) ];
+  Δsdt_m := λ _ _, [(IntT, BoolT) ];
+}.
+
+Local Instance SDTCS : SDTClassSpec.
+Proof.
+  split.
+  - move =>>; rewrite list_lookup_singleton_Some => [[? <-]]; by constructor.
+  - move =>>; rewrite list_lookup_singleton_Some => [[? <-]]; by constructor.
+  - move =>> ?; rewrite list_lookup_singleton_Some => [[? <-]]; by constructor.
+  - move =>> ?; rewrite list_lookup_singleton_Some => [[? <-]]; by constructor.
+  - move =>>; rewrite list_lookup_singleton_Some => [[? <-]]; by constructor.
+  - move =>>; rewrite list_lookup_singleton_Some => [[? <-]]; by constructor.
+Qed.
+
+Lemma has_method_C_f: has_method "f" "C" "C" f.
+Proof. by repeat econstructor; eauto. Qed.
+
+Lemma has_method_D_f: has_method "f" "D" "D" f2.
+Proof. by repeat econstructor; eauto. Qed.
+
+Lemma has_method_D_g: has_method "g" "D" "D" g.
+Proof. by repeat econstructor; eauto. Qed.
+
+Lemma has_method_Main_problem: has_method "problem" "Main" "Main" problem.
+Proof. by repeat econstructor; eauto. Qed.
+
+Lemma has_method_Main_main: has_method "main" "Main" "Main" main.
+Proof. by repeat econstructor; eauto. Qed.
+
+Lemma has_fields_C : has_fields "C" ∅.
+Proof.
+  move => f vis fty orig; split => h.
+  - inv h.
+    + rewrite /pdefs /= lookup_insert in H.
+      by simplify_eq.
+    + by rewrite /pdefs /= lookup_insert in H; simplify_eq.
+  - by rewrite lookup_empty in h.
+Qed.
+
+Lemma has_fields_D : has_fields "D" ∅.
+Proof.
+  move => f vis fty orig; split => h.
+  - inv h.
+    + rewrite /pdefs /= lookup_insert_ne in H; last done.
+      rewrite lookup_insert in H.
+      by simplify_eq.
+    + rewrite /pdefs /= lookup_insert_ne in H; last done.
+      rewrite lookup_insert in H; simplify_eq.
+      rewrite /D /= in H1; simplify_eq.
+      move : has_fields_C => hf0.
+      apply hf0 in H2.
+      by rewrite lookup_empty in H2.
+  - by rewrite lookup_empty in h.
+Qed.
+
+Lemma has_fields_Main : has_fields "Main" ∅.
+Proof.
+  move => f vis fty orig; split => h.
+  - inv h.
+    + rewrite /pdefs /= lookup_insert_ne in H; last done.
+      rewrite lookup_insert_ne in H; last done.
+      rewrite lookup_insert in H.
+      by simplify_eq.
+    + rewrite /pdefs /= lookup_insert_ne in H; last done.
+      rewrite lookup_insert_ne in H; last done.
+      rewrite lookup_insert in H; by simplify_eq.
+  - by rewrite lookup_empty in h.
+Qed.
+
+(* TODO: name this *)
+Definition ΔC :=
+  let n := length C.(generics) in
+  let σ := gen_targs n in
+  (ThisT, ClassT false "C" σ) :: C.(constraints).
+
+Lemma wf_mdef_ty_C_f: wf_mdef_ty "C" ΔC 0 f.
+Proof.
+  rewrite /wf_mdef_ty.
+  exists f.(methodargs).
+  repeat split.
+  - apply map_Forall_lookup => k tk. 
+    rewrite /f /=.
+    by rewrite lookup_singleton_Some => [[? <-]].
+  - rewrite /f /=.
+    by apply SkipTy.
+  - rewrite /f /=.
+    by apply NullTy.
+Qed.
+
+Definition ΔD :=
+  let n := length D.(generics) in
+  let σ := gen_targs n in
+  (ThisT, ClassT false "D" σ) :: D.(constraints).
+
+Lemma wf_mdef_ty_D_f: wf_mdef_ty "D" ΔD 0 f2.
+Proof.
+  rewrite /wf_mdef_ty /f2 /=.
+  exists (<[ "$_" := NullT]> f2.(methodargs)).
+  repeat split.
+  - apply map_Forall_insert_2; first by constructor.
+    apply map_Forall_singleton; by constructor.
+  - rewrite /f2 /=.
+    change {["$_" := NullT; "$in" := ThisT]}
+    with (<["$_" := subst_fty false "D" [] g.(methodrettype)]> f2.(methodargs)).
+    apply CallPubInexactTy with (orig := "D").
+    + eapply ESubTy.
+      * constructor.
+        by rewrite lookup_insert.
+      * by econstructor.
+      * by econstructor.
+      * by econstructor.
+      * apply SubConstraint.
+        by set_solver.
+    + by apply HasMethod with (cdef := D).
+    + done.
+    + by rewrite /g /= !dom_insert_L !dom_empty_L.
+    + move => t0 σ0 h0 k ty arg => /=.
+      rewrite lookup_insert_Some => [[ [<- <-] | [? h]]]; last by simplify_eq.
+      rewrite lookup_insert => [[<-]].
+      by rewrite /subst_fty /= subst_ty_gen_targs.
+  - by apply NullTy.
+Qed.
+
+Lemma wf_mdef_ty_D_g: wf_mdef_ty "D" ΔD 0 g.
+Proof.
+  rewrite /wf_mdef_ty.
+  exists g.(methodargs).
+  repeat split.
+  - apply map_Forall_lookup => k tk. 
+    rewrite /g /=.
+    by rewrite lookup_singleton_Some => [[? <-]].
+  - rewrite /g /=.
+    by apply SkipTy.
+  - rewrite /g /=.
+    by apply NullTy.
+Qed.
+
+Definition ΔM :=
+  let n := length Main.(generics) in
+  let σ := gen_targs n in
+  (ThisT, ClassT false "Main" σ) :: Main.(constraints).
+
+Definition Γmain : stringmap lang_ty :=
+  (<[ "$c" := ClassT true "C" [] ]>
+  (<[ "$d" := ClassT true "D" [] ]> main.(methodargs))).
+
+Lemma wf_mdef_ty_main: wf_mdef_ty "main" ΔM 0 main.
+Proof.
+  rewrite /wf_mdef_ty.
+  exists (<[ "$tmp" := NullT]> Γmain).
+  repeat split.
+  - apply map_Forall_insert_2; first by constructor.
+    apply map_Forall_insert_2; first by repeat econstructor.
+    apply map_Forall_insert_2; first by repeat econstructor.
+    by apply map_Forall_empty.
+  - rewrite /main /=.
+    eapply SeqTy.
+    { eapply NewTy => //.
+      - by repeat econstructor.
+      - by repeat econstructor.
+      - by econstructor.
+      - by exact has_fields_D.
+      - by rewrite !dom_empty_L.
+    }
+    eapply SeqTy.
+    { eapply NewTy => //.
+      - by repeat econstructor.
+      - by repeat econstructor.
+      - by econstructor.
+      - by exact has_fields_C.
+      - by rewrite !dom_empty_L.
+    }
+    change (<["$tmp" := NullT]> Γmain)
+    with (<["$tmp" := subst_fty false "Main" [] problem.(methodrettype)]>  Γmain).
+    apply CallPubInexactTy with (orig := "Main").
+    + eapply ESubTy.
+      * by constructor.
+      * by econstructor.
+      * by econstructor.
+      * by econstructor.
+      * apply SubConstraint.
+        by set_solver.
+    + by apply HasMethod with (cdef := Main).
+    + done.
+    + by rewrite /problem /= !dom_insert_L !dom_empty_L.
+    + move => t0 σ0 h0 k ty arg => /=.
+      rewrite lookup_insert_Some => [[ [<- <-] | [? h]]].
+      * rewrite lookup_insert => [[<-]].
+        rewrite /subst_fty /=.
+        eapply ESubTy.
+        -- constructor.
+           by set_solver.
+        -- rewrite /subst_fty /=.
+           by econstructor.
+        -- rewrite /subst_fty /=.
+           by econstructor.
+        -- rewrite /subst_fty /=.
+           by econstructor.
+        -- rewrite /subst_fty /=.
+           apply SubTrans with (ClassT false "D" []).
+           { by apply SubExact with D. }
+           change (ClassT false "C" []) with (ClassT false "C" (subst_ty [] <$> [])).
+           apply SubClass with D => //.
+           by apply ExtendsUsing with D.
+      * apply lookup_singleton_Some in h as [<- <-].
+        rewrite lookup_insert_ne //.
+        rewrite lookup_insert => [[ <- ]] /=.
+        rewrite /subst_fty /=.
+        eapply ESubTy.
+        -- constructor.
+           by set_solver.
+        -- rewrite /subst_fty /=.
+           by econstructor.
+        -- rewrite /subst_fty /=.
+           by econstructor.
+        -- rewrite /subst_fty /=.
+           by econstructor.
+        -- by apply SubExact with C.
+  - by apply NullTy.
+Qed.
+
+Lemma wf_mdef_ty_problem: wf_mdef_ty "problem" ΔM 0 problem → False.
+Proof.
+  rewrite /wf_mdef_ty /problem /=.
+  case => Γf.
+  case => hwfΓf.
+  case => hc _.
+  inv hc.
+  - apply var_has_ty_inv in H3.
+    rewrite lookup_insert in H3.
+
+
+Qed.
+
+Lemma wf_mdef_ty_problem: wf_mdef_ty "problem" ΔM 0 problem.
+Proof.
+  rewrite /wf_mdef_ty.
+  exists (<[ "$_" := NullT]> problem.(methodargs)).
+  repeat split.
+  - apply map_Forall_insert_2; first by constructor.
+    apply map_Forall_insert_2; first by repeat econstructor.
+    apply map_Forall_insert_2; first by repeat econstructor.
+    by apply map_Forall_empty.
+  - rewrite /problem /=.
+    change ({["$_" := NullT; "$c0" := ClassT false "C" []; "$c1" := ClassT false "C" []]})
+    with (<["$_" := subst_fty false "C" [] f.(methodrettype)]> problem.(methodargs)).
+    apply CallPubInexactTy with "C".
+    + by apply GenTy.
+    + by econstructor.
+    + done.
+    + by rewrite /f /= !dom_insert_L !dom_empty_L.
+    + rewrite /f => t0 σ0 h0 k ty arg /=.
+      rewrite lookup_singleton_Some => [[<- <-]].
+      rewrite lookup_insert /subst_fty => [[ <- ]] /=.
+      rewrite subst_ty_gen_targs; last done.
+      (* not possible *)
+  - by apply NullTy.
+Qed.
+
+Print Assumptions wf_mdef_ty_problem.
